theories/L/Complexity/Reductions/TMGenNP/mTM_to_singleTapeTM.v
@@ -11,28 +11,574 @@ From Undecidability.L.Complexity  Require Import LMGenNP TMGenNP_fixed_mTM.
 
 From Undecidability.TM.Single Require EncodeTapes StepTM DecodeTapes. (** In emacs: coq-prefer-top-of-conclusion: t; *)
 
+Unset Printing Coercions.
+From Coq.ssr Require ssrfun.
+Module Option := ssrfun.Option.
 
 Module MultiToMono.
   Section multiToMono.
 
+    (** We can simulate any machine while first testing that we indeed work on a valid n-tape encoding *)
+
     Import EncodeTapes DecodeTapes Single.StepTM ProgrammingTools Combinators Decode.
-    Context (sig F:finType) (n:nat) (M__multi : pTM sig F (S n)).
+    Context (sig F:finType) (n:nat) (M__multi : pTM sig F n).
 
     Definition M : pTM ((sigList (sigTape sig)) ^+) (option F) 1 :=
-      If (CheckTapeContains.M (CheckEncodesTapes.M (S n)))
-         (Relabel (ToSingleTape M__multi) Some)
+      If (CheckTapeContains.M (CheckEncodesTapes.M n))
+         (Move L;;If (Relabel ReadChar (Option.apply (fun _ => false) true))
+                     (Move R;;Relabel (ToSingleTape M__multi) Some)
+                     (Return Nop None))
          (Return Nop None).
 
-    
+    Definition Rel : pRel ((sigList (sigTape sig)) ^+) (option F) 1 :=
+      fun t '(y,t') => match y with
+                      None => ~ exists (v : tapes sig n), StepTM.contains_tapes t[@Fin0] v
+                    | Some y => exists (v v': tapes sig n), StepTM.contains_tapes t[@Fin0] v
+                                                      /\ StepTM.contains_tapes t'[@Fin0] v'
+                                                      /\ Canonical_Rel M__multi v (y,v')
+                    end.
 
+    Lemma Realises : M ⊨ Rel .
+    Proof.
+      intros H__multi.
+      eapply Realise_monotone.
+      {unfold M. TM_Correct.
+       -apply CheckTapeContains.Realises. now apply CheckEncodesTapes.Realises. exact _.
+       -eapply ToSingleTape_Realise', Canonical_Realise.
+      }  
+      intros t (y,t'). cbn in *.
+      intros [H|H];unfold Rel;cbn.
+      2:{ destruct H as (?&([Henc]&_)&->&_&<-). intros (v&Hv). hnf in Hv. inversion Henc. apply H.
+          exists v,[]. rewrite Hv. now rewrite Encode_map_id. } 
+      destruct H as (?&[[Henc] <-]&_&t1&Ht1&H). 2:easy.
+      destruct H as [H|H].
+      2:{ destruct H as (?&(?&?&->&<-)&->&_&<-). rewrite Ht1 in H. intros (v&Ht). hnf in Ht.
+          rewrite Ht in H. now cbn in H. }
+      destruct H as (?&(?&Hc1&->&->)&(_&t2&Ht2&y'&->&Hm)).
+      rewrite Ht1 in Ht2. destruct (current t1[@Fin0]) eqn:Hc1';inv Hc1.
+      inv Henc. rename H into Henc. destruct Henc as (x'&t__L&Henc). rewrite Encode_map_id in Henc.
+      erewrite tape_move_left_right in Ht2. 2:now rewrite Henc.
+      rewrite Ht2 in *. clear Ht2 t2. rewrite Ht1 in *. clear Ht1 t1.
+      destruct t__L. 2:now rewrite Henc in Hc1'.
+      specialize Hm with (1:=Henc) as (?&(?&?&?&<-&<-)&?).
+      do 3 eexists. exact Henc. split. eauto.
+      unfold Canonical_T;eauto. 
+    Qed.
 
+    Context (T__multi : tRel sig n).
+
+    Definition Ter : tRel ((sigList (sigTape sig)) ^+) 1 :=
+      fun t k  => exists (k' k__sim: nat), (forall (v : tapes sig n),
+                                   StepTM.contains_tapes t[@Fin0] v
+                                   -> T__multi v k__sim
+                                     /\ Loop_steps (start (projT1 M__multi)) v k__sim <= k')
+                               /\ ((| right t[@Fin0] |)*4*(n+1) + n*16 + 27 + k') <= k .
+
+    Lemma Terminates  : projT1 M__multi ↓ T__multi -> projT1 M ↓ Ter.
+    Proof.
+      intros H__multi.
+      eapply TerminatesIn_monotone.
+      {unfold M. TM_Correct.
+       -apply CheckTapeContains.Realises. now apply CheckEncodesTapes.Realises. exact _.
+       -eapply CheckTapeContains.Terminates. now apply CheckEncodesTapes.Realises. apply CheckEncodesTapes.Terminates.
+       -eapply ToSingleTape_Terminates'. eassumption.
+      }  
+      intros t k (k'&k__sim&Hk__sim&Hk). infTer 2. infTer 2. hnf. reflexivity.
+      split. shelve.
+      intros ? b [Henc Hbeq]. destruct b. 2:now apply Nat.le_0_l.
+      infTer 4. intros t1 [] Ht1. cbn in Ht1.
+      infTer 4. cbn. intros t2 b (?&Hb&->&->).
+      destruct b. 2:now apply Nat.le_0_l.
+      infTer 4. intros t2 _ Ht2. hnf.
+      destruct Henc. inv H. rename H0 into Henc. destruct Henc as (v&t__L&Heq).
+      rewrite Ht1 in Ht2. specialize (Hbeq eq_refl). subst tout. cbn in *.
+      rewrite Heq in Ht1. rewrite Ht1 in Hb. destruct t__L;inv Hb. rewrite Heq in Ht2. cbn in Ht2.
+      rewrite Ht2. clear Ht2 Ht1 t1 t2.
+      edestruct Hk__sim as (H__k&Hk__sim').  1:{ hnf. rewrite Heq. now rewrite map_id. }
+      eexists v,_. split. 1:{ hnf. now rewrite map_id. }
+      split. eassumption. eassumption.
+      Unshelve. cbn - [plus mult]. rewrite CheckEncodesTapes.length_right_tape_move_right. cbn - [plus mult].
+      ring_simplify.
+      transitivity ((| right t[@Fin0] |)*4*(n+1) + n*16 + 27 + k'). cbn - [plus mult].
+      nia. exact Hk. 
+    Qed.
+(*
+    Definition Ter' : tRel ((sigList (sigTape sig)) ^+) 1 :=
+      fun t k  => exists (k' k__sim: nat), (forall (v : tapes sig n),
+                                   StepTM.contains_tapes t[@Fin0] v
+                                   -> Canonical_T (projT1 M__multi) v k__sim
+                                     /\ Loop_steps (start (projT1 M__multi)) v k__sim <= k')
+                               /\ ((| right t[@Fin0] |)*4*(n+1) + n*16 + 27 + k') <= k .
+
+    Local Arguments Canonical_T : simpl never. 
+    Lemma Terminates'  : projT1 M ↓ Ter'.
+    Proof.
+      intros H__multi.
+      eapply TerminatesIn_monotone.
+      {unfold M. TM_Correct.
+       -apply CheckTapeContains.Realises. now apply CheckEncodesTapes.Realises. exact _.
+       -eapply CheckTapeContains.Terminates. now apply CheckEncodesTapes.Realises. apply CheckEncodesTapes.Terminates.
+       -eapply ToSingleTape_Terminates'. eapply Canonical_TerminatesIn.
+      }  
+      intros t k (k'&k__sim&Hk__sim&Hk). infTer 2. infTer 2. hnf. reflexivity.
+      split. shelve.
+      intros ? b [Henc Hbeq]. destruct b. 2:now apply Nat.le_0_l.
+      infTer 4. intros t1 [] Ht1. cbn in Ht1.
+      infTer 4. cbn. intros t2 b (?&Hb&->&->).
+      destruct b. 2:now apply Nat.le_0_l.
+      infTer 4. intros t2 _ Ht2. hnf.
+      destruct Henc. inv H. rename H0 into Henc. destruct Henc as (v&t__L&Heq).
+      rewrite Ht1 in Ht2. specialize (Hbeq eq_refl). subst tout. cbn in *.
+      rewrite Heq in Ht1. rewrite Ht1 in Hb. destruct t__L;inv Hb. rewrite Heq in Ht2. cbn in Ht2.
+      rewrite Ht2. clear Ht2 Ht1 t1 t2.
+      edestruct Hk__sim as (H__k&Hk__sim').  1:{ hnf. rewrite Heq. now rewrite map_id. }
+      eexists v,_. split. 1:{ hnf. now rewrite map_id. }
+      split. eassumption. eassumption.
+      Unshelve. cbn - [plus mult]. rewrite CheckEncodesTapes.length_right_tape_move_right. cbn - [plus mult].
+      ring_simplify.
+      transitivity ((| right t[@Fin0] |)*4*(n+1) + n*16 + 27 + k'). cbn - [plus mult].
+      nia. exact Hk. 
+    Qed. 
+    *)
   End multiToMono.
 End MultiToMono.
+Arguments MultiToMono.Rel : simpl never.
+Arguments MultiToMono.Ter : simpl never.
 
-Lemma LMGenNP_to_TMGenNP_mTM (sig:finType) (n:nat) `{R__sig : registered sig}  (M : mTM sig (S n)):
-  exists sig' `{R__sig' : registered sig'} (M' : mTM sig 1),
+
+(*****************************************************************)
+(* Module Diverge.                                               *)
+(*   Section Diverge.                                            *)
+(*                                                               *)
+(*     Import ProgrammingTools While.                            *)
+(*     Context {sig:finType} {n:nat}.                              *)
+(*     Definition M : pTM sig unit n := While (Return Nop None). *)
+(*                                                               *)
+(*     Lemma Realises : M ⊨ (fun _ _ => False).                         *)
+(*     Proof.                                                    *)
+(*       eapply Realise_monotone. 1:{unfold M. TM_Correct. }     *)
+(*       apply WhileInduction. all:cbn. all:easy.                *)
+(*     Qed.                                                      *)
+(*   End Diverge.                                                *)
+(* End Diverge.                                                  *)
+(*****************************************************************)
+
+Import LTactics GenEncode CodeTM EncodeTapes.
+  
+Run TemplateProgram (tmGenEncode "boundary_enc" boundary).
+Hint Resolve boundary_enc_correct : Lrewrite.
+
+Section sigList.
+  Context (sig : Type) `{H:registered sig}.
+  Run TemplateProgram (tmGenEncode "sigList_enc" (sigList sig)).
+
+  Global Instance term_sigList_X : computableTime' (@sigList_X sig) (fun _ _ => (1,tt)).
+  Proof. extract constructor. solverec.
+  Qed.
+
+End sigList.
+Hint Resolve sigList_enc_correct : Lrewrite.
+
+
+Section sigTape.
+  Context (sig : Type) `{H:registered sig}.
+  Run TemplateProgram (tmGenEncode "sigTape_enc" (sigTape sig)).
+End sigTape.
+Hint Resolve sigTape_enc_correct : Lrewrite.
+
+
+From Undecidability Require Import Datatypes.Lists.
+
+Section LMGenNP_to_TMGenNP_mTM.
+  Import EncodeTapes DecodeTapes Single.StepTM ProgrammingTools Combinators Decode.
+  Import LTactics LSum LProd LVector LNat Lists.
+
+  Context (sig:finType) (n:nat) `{R__sig : registered sig}  (M : mTM sig (S n)).
+
+  
+  Definition putFirstAtEnd n: Vector.t (Fin.t (S n)) (S n):=
+    tabulate (fun i => match lt_dec (S (proj1_sig (Fin.to_nat i))) (S n) with
+                      Specif.left H => Fin.of_nat_lt H
+                    | _ => Fin.F1
+                    end).
+  Arguments putFirstAtEnd : simpl never.
+
+  Definition putEndAtFirst n': Vector.t (Fin.t (S n')) (S n'). 
+    refine (tabulate (fun i => match Fin.to_nat i with
+                    | exist _ 0 H => Fin.of_nat_lt (Nat.lt_succ_diag_r n')
+                    | exist _ n' H => Fin.of_nat_lt (p:=n'-1) _
+                            end )). abstract nia.
+  Defined.
+  Arguments putEndAtFirst : simpl never.
+
+  Section printFin.
+    Local Arguments Fin.t : clear implicits.
+    Local Arguments Fin.FS : clear implicits.
+    Local Arguments Fin.F1 : clear implicits.
+    Local Arguments Vector.cast : clear implicits.
+
+    Lemma putFirstAtEnd_dupfree m: dupfree (putFirstAtEnd m).
+    Proof.
+      clear_all. apply dupfree_tabulate_injective.
+      intros i j. destruct (Fin.to_nat i) as [i' Hi] eqn:eqi. destruct (Fin.to_nat j) as [j' Hj] eqn:eqj .
+      cbn. 1:do 2 destruct lt_dec. 2,3:easy.
+      2:{ intros _. apply Fin.to_nat_inj. rewrite eqi. rewrite eqj. cbn. clear eqi eqj. nia. }
+      intros H%Fin.FS_inj. apply Fin.to_nat_inj.
+      rewrite eqi,eqj. cbn. specialize (lt_S_n _ _ l) as H1. specialize (lt_S_n _ _ l0) as H2.
+      erewrite <- (Fin.of_nat_ext H1), <- (Fin.of_nat_ext H2) in H.
+      apply(f_equal Fin.to_nat) in H. rewrite !Fin.to_nat_of_nat in H.
+      now inv H.
+    Qed.
+    
+    Lemma putEndAtFirst_dupfree m: dupfree (putEndAtFirst m).
+    Proof.
+      clear_all. apply dupfree_tabulate_injective.
+      intros i j.
+      destruct (Fin.to_nat i) eqn:?;destruct (Fin.to_nat j) eqn:?; cbn in *.
+      eassert (H'1:=Heqs). assert (H'2:=Heqs0).
+      erewrite <- (Fin.of_nat_to_nat_inv i) in Heqs. erewrite <- (Fin.of_nat_to_nat_inv j) in Heqs0. 
+      rewrite Fin.to_nat_of_nat in Heqs. rewrite Fin.to_nat_of_nat in Heqs0. inversion Heqs; inversion Heqs0.
+            destruct (fin_destruct_S i) as [ (i'&->) | ->]; destruct (fin_destruct_S j) as [ (j'&->) | ->].
+            all:try change (Fin.FS m i') with (Fin.R 1 i') in *; try change (Fin.FS m j') with (Fin.R 1 j') in *.
+            all:change (S m) with (1+m) in *.
+            all: rewrite ?Fin.R_sanity in H0;rewrite ?Fin.R_sanity in H1. all: subst;cbn.
+            all:intros Heq%(f_equal Fin.to_nat).
+            all:rewrite !Fin.to_nat_of_nat in Heq. 
+            all:inversion Heq as [H2]. all:try rewrite ?Nat.sub_0_r in H2.
+            all:try apply Fin.to_nat_inj in H2. all:try easy.
+      -clear - l H2.  nia.
+      -clear - l0 H2.  nia.
+    Qed.
+    
+  End printFin.
+  
+  Definition M__mono : pTM ((sigList (sigTape sig)) ^+) unit 1 :=
+    If (Move R ;; Relabel (MultiToMono.M (LiftTapes (M;(fun _ => tt)) (putEndAtFirst n) )) (Option.apply (fun _ => true) false))
+       Nop
+       Diverge.
+
+  Local Arguments Canonical_Rel : simpl never. 
+  Lemma Realises__mono:
+    M__mono ⊨(fun tin '(_,tout) =>
+              exists v v' : tapes sig (S n),
+                contains_tapes (tape_move_right tin[@Fin0]) v /\
+                contains_tapes tout[@Fin0] v' /\
+                Canonical_Rel (LiftTapes (existT (fun x : mTM sig (S n) => states x -> unit) M (fun _ : states M => tt)) (putEndAtFirst n)) v
+                              (tt, v')).
+  Proof.
+    eapply Realise_monotone.
+    { unfold M__mono. TM_Correct. apply MultiToMono.Realises. } cbn.
+    intros tin ([],tout). cbn. intros [H|H].
+    2:now decompose record H.
+    destruct H as (?&([]&t1&Ht1&b&Hb&H__mono)&<-). destruct b as [ [] | ] ;inv Hb.
+    hnf in H__mono. cbn - [Canonical_Rel]in *|-*. rewrite Ht1 in *|-*. easy.
+  Qed.
+  
+    Lemma Terminates_False sig' n' (M' : mTM sig' n'): M' ↓ (fun _ _ => False).
+  Proof.
+    easy.
+  Qed.
+  
+
+  Lemma Terminates__mono:
+    projT1 M__mono ↓ (fun t k => exists (v : tapes _ (S n)) k',
+                        contains_tapes (tape_move_right t[@Fin0]) v
+                        /\ MultiToMono.Ter (LiftTapes (existT _ M (fun _  => tt)) (putEndAtFirst n))
+                                          (LiftTapes_T (putEndAtFirst n) (Canonical_T M))
+                                          [|(tape_move_right t[@Fin0])|] k'
+                        /\ k' + 3 <= k).
+  Proof.
+    eapply TerminatesIn_monotone.
+    { unfold M__mono. TM_Correct.
+      -apply MultiToMono.Realises.
+      -eapply MultiToMono.Terminates. apply LiftTapes_Terminates. apply putEndAtFirst_dupfree. eapply Canonical_TerminatesIn.
+      -apply Terminates_False.
+    }
+    intros tin k (v&k'&Hv&HT&Hk). cbn.
+    infTer 7. intros t1 _ Ht1. unfold tapes in *. destruct_vector;cbn in *. subst h. apply HT. shelve.
+    intros tout b (?&t1&Ht1&[[]| ]&->&Hr). all:cbn. 2:{ apply Hr. cbn in *. rewrite <- Ht1 in *. easy. } reflexivity.
+    Unshelve.
+    { rewrite <- Hk. nia. } (*
+    hnf in Hr. destruct Hr as (v0&v'&Hv0&Hv'&Hr). replace v0 with v in * by admit.
+    hnf in Hr. cbnunfold LiftTapes in Hr.  cbn in Hr.
+    (*TODO: move trivial relation in Realisation so we get that M terminated if M__Mono halted. *)
+    destruct r
+    2:now decompose record H.
+    destruct H as (?&(b&Hf&H)&<-).
+    destruct b as [[]| ];inv Hf. 
+    destruct H as (v&v'&Hv&Hv'&HR&_).
+    do 3 eexists. 2:split. all:eassumption. *)
+  Qed.
+  
+  
+
+  (*MOVE*)
+  Lemma sizeOfTape_encodeTape sig' (t : tape sig') :
+  | encode_tape t | = let l := sizeOfTape t in if 0 =? l then 1 else 2 + sizeOfTape t.
+  Proof.
+    destruct t;cbn - [Nat.eqb].
+    all:repeat (autorewrite with list;cbn [length]).
+    1:easy.
+    2,3:rewrite !Nat.add_succ_r. all:cbn [Nat.eqb]. all:nia.
+  Qed.
+
+  
+  Lemma sizeOfTape_encodeTape_le sig' (t : tape sig') :
+  | encode_tape t | <= 2 + sizeOfTape t.
+  Proof.
+    rewrite sizeOfTape_encodeTape. cbn;destruct _;nia.
+  Qed.
+
+  Import EqBool.
+
+  Lemma encode_list_concat sigX X (cX : codable sigX X) l:
+    encode_list cX l = concat (map (fun t => sigList_cons :: map sigList_X (encode t)) l) ++[sigList_nil].
+  Proof.
+    induction l;cbn. reflexivity.
+    rewrite IHl. cbn. now autorewrite with list.
+  Qed.
+
+  Lemma list_eq_nth_error X (xs ys : list X) :
+    (forall n, nth_error xs n = nth_error ys n) -> xs = ys.
+  Proof.
+    induction xs in ys|-*;destruct ys;cbn;intros H. 1:easy. 1-2:now specialize (H 0).
+    generalize (H 0).  intros [= ->]. erewrite IHxs. easy. intros n'. now specialize (H (S n')).
+  Qed.
+
+  Lemma vector_nth_error X n' i (xs : Vector.t X n') :
+    nth_error (Vector.to_list xs) i = match lt_dec i n' with
+                                        Specif.left H => Some (Vector.nth xs (Fin.of_nat_lt H))
+                                      | _ => None
+                                      end.
+  Proof.
+    clear. rewrite <- vector_to_list_correct. induction xs in i|-*. now destruct i.
+    cbn in *. destruct i;cbn. easy. rewrite IHxs. do 2 destruct lt_dec. 4:easy. now symmetry;erewrite Fin.of_nat_ext. all:exfalso;nia. 
+  Qed.
+    
+
+  Lemma putFirstAtEnd_to_list X n' (x:X) xs:
+    (Vector.to_list (select (putFirstAtEnd n') (x ::: xs))) = Vector.to_list xs ++ [x].
+  Proof.
+    clear. apply list_eq_nth_error. intros i.
+    rewrite !vector_nth_error. destruct lt_dec.
+    { rewrite select_nth. unfold putFirstAtEnd. rewrite nth_tabulate,Fin.to_nat_of_nat;cbn.
+      destruct lt_dec.
+      -erewrite nth_error_app1. 2:now rewrite TMunflatten.vector_to_list_length.
+       cbn. rewrite vector_nth_error. destruct lt_dec. 2:exfalso;nia.
+       erewrite Fin.of_nat_ext. reflexivity.
+      -cbn. rewrite nth_error_app2. all:rewrite TMunflatten.vector_to_list_length. 2:nia. replace (i-n') with 0 by nia. easy.
+    }
+    symmetry. apply nth_error_None. erewrite app_length, TMunflatten.vector_to_list_length. cbn;nia.
+  Qed.
+
+  Lemma putEnd_invL X (v : Vector.t X _) :
+    select (putEndAtFirst n) (select (putFirstAtEnd n) v) = v.
+  Proof.
+    apply Vector.eq_nth_iff. intros i ? <-. rewrite !select_nth.
+    f_equal. 
+    unfold putEndAtFirst,putFirstAtEnd. rewrite !nth_tabulate.
+    destruct (fin_destruct_S i) as  [(i'&->) | ->].
+    2:{ cbn. rewrite Fin.to_nat_of_nat. cbn. destruct lt_dec. now exfalso;nia. easy. }
+    eapply Fin.to_nat_inj.
+    remember (Fin.to_nat (Fin.FS i')) as i0 eqn:H. set (tmp:=proj1_sig i0).
+    rewrite (sig_eta i0). subst tmp i0. cbn.
+    destruct (Fin.to_nat i') eqn:H.
+    cbn. rewrite Fin.to_nat_of_nat;cbn. destruct lt_dec;cbn.
+    -rewrite (sig_eta (Fin.to_nat _)). cbn. rewrite Fin.to_nat_of_nat. cbn. nia.
+    -clear H. nia.
+  Qed.
+
+  
+  Lemma right_sizeOfTape sig' (t:tape sig') :
+    length (right t) <= sizeOfTape t.
+  Proof.
+    destruct t;cbn. all:autorewrite with list;cbn. all:nia.
+  Qed.
+  
+
+
+  From Undecidability Require Import MultiUnivTimeSpaceSimulation.
+  Lemma size_list X sigX (cX: codable sigX X) (l:list X) :
+    size l = sumn (map size l) + length l + 1.
+  Proof.
+    unfold size. cbn. rewrite encode_list_concat.
+    rewrite app_length, length_concat, map_map. cbn.
+    change S with (fun x => 1 + x). rewrite sumn_map_add,sumn_map_c. setoid_rewrite map_length.
+    cbn.  nia.
+  Qed.
+
+  Lemma concat_eq_inv_borderL X isBorder xs R__L ys b (R__R : list X):
+    (forall x, x el xs -> exists hd tl, x = hd::tl /\ isBorder hd /\ forall c, c el tl -> ~isBorder c) ->
+    (forall x, x el ys -> exists hd tl, x = hd::tl /\ isBorder hd /\ forall c, c el tl -> ~isBorder c) ->
+    (forall x, x el R__R -> ~isBorder x) ->
+    isBorder b ->
+    concat xs ++ b::R__L = concat ys++R__R ->
+    (forall i, i < length xs -> nth_error xs i = nth_error ys i) /\ b::R__L = concat (skipn (length xs) ys) ++ R__R.
+  Proof.
+    clear. induction xs as [ | x xs] in ys|-*;intros HL HR HRR Hb Heq.
+    { cbn in *. easy. }
+    destruct ys as [ |y ys].
+    { exfalso. cbn in Heq. subst R__R.
+      destruct (HL x) as (?&?&->&?&?). easy. eapply HRR. 2:easy. cbn;easy. }
+    cbn in Heq. autorewrite with list in Heq.
+    destruct (HL x) as (x__hd&x__tl&->&Hxhd&Hxtl). easy.
+    destruct (HR y) as (y__hd&y__tl&->&_&Hytl). easy.
+    cbn in *. 
+    revert Heq. intros [= <- Heq].
+    replace y__tl with x__tl in *.
+    2:{ induction x__tl as [ | x' xtl] in y__tl,Heq,HL,HR,Hytl,Hxtl|-*.
+        -destruct y__tl. easy. cbn in Heq. destruct xs.
+         +now edestruct (Hytl x);inv Heq.
+         +edestruct (HL l) as (?&?&->&?&?). easy. inv Heq. now edestruct Hytl.
+        -destruct y__tl.
+         2:{ inv Heq. f_equal. eapply IHxtl. 3-5:cbn;intros;auto.
+             all:intros z [<-| ].  all:now eauto 7. 
+         }
+         exfalso. destruct ys. 2:{ edestruct (HR l) as (?&?&->&?&?). easy. inv Heq. cbn in *. now eapply Hxtl. }
+         cbn in Heq. 
+         inv Heq. eapply HRR. 2:exact Hb. eauto 10.
+    }
+    apply app_inv_head in Heq. apply IHxs in Heq.  2-5:now eauto 7.
+    destruct Heq as (IH&->). split. 2:easy.
+    intros [] ?. easy. cbn. apply IH. nia.
+  Qed.
+
+  Lemma vector_app_to_list X k k' (xs : Vector.t X k) (ys : Vector.t X k'):
+    vector_to_list (Vector.append xs ys) = vector_to_list xs ++ vector_to_list ys.
+  Proof.   
+    induction xs. easy. cbn. congruence.
+  Qed.
+
+  Lemma putEndAtFirst_to_list X n' v (ts:X) v0:
+    Vector.to_list v ++ [ts] = Vector.to_list v0 ->
+    select (putEndAtFirst n') v0 = ts ::: v.
+  Admitted.
+
+  Instance term_concat X `{registered X}: computableTime' (@concat X) (fun l _ => (cnst ("todo",l),tt)).
+  Admitted.
+
+  
+  Instance term_encode_tape X `{registered X}: computableTime' (@encode_tape X) (fun l _ => (cnst ("todo: encode_tape",l),tt)).
+  Admitted.
+
+  Lemma contains_tapes_inj (sig' : finType) n' t (v v' : tapes sig' n'):
+    contains_tapes t v -> contains_tapes t v' -> v = v'.
+  Proof.
+    unfold contains_tapes. intros -> [= eq]. apply app_inv_tail in eq. apply map_injective in eq. 2:congruence.
+    eassert (H':=encode_prefixInjective (t:=[]) (t':=[])). rewrite !app_nil_r in H'. apply H' in eq. easy.
+  Qed.
+  
+  Local Arguments loopM : clear implicits.
+  Local Arguments loopM {_ _ } _ _ _. 
+  Lemma LMGenNP_to_TMGenNP_mTM :
     restrictBy (HaltsOrDiverges_fixed_mTM M) (TMGenNP_fixed_mTM M)
-               ⪯p unrestrictedP (TMGenNP_fixed_singleTapeTM M').
-Proof.
+               ⪯p unrestrictedP (TMGenNP_fixed_singleTapeTM (projT1 M__mono)).
+  Proof.
+    evar (f__steps : nat -> nat -> nat -> nat). unfold TMGenNP_fixed_mTM. unfold TMGenNP_fixed_singleTapeTM. cbn.
+    set (t__start:=fun (ts : tapes sig n) => inl START::concat (map (fun t => inr (sigList_cons)::map (fun s => inr (sigList_X s)) (encode_tape t)) (Vector.to_list ts))++[inr (sigList_cons)]).
+    eapply reducesPolyMO_intro_restrictBy with
+        (f:=fun '(ts,maxSize,steps) => (t__start ts
+                                     ,3 + if eqb 0 maxSize then 0 else 1 + maxSize
+                                     ,f__steps steps (sizeOfmTapes ts) maxSize+ 3)).
+    2:{ intros [[v maxSize] steps]. unfold HaltsOrDiverges_fixed_mTM. intros H_HaltOrDiv.
+        split. easy. split.
+        -intros (t1&Ht1&s__end&Hs__end). cbn.
+         eexists _,(map (fun c => inr (sigList_X c)) (encode_tape t1) ++ [inr sigList_nil;inl STOP]). split. now subst t__start. 
+         split. 1:{ autorewrite with list. rewrite sizeOfTape_encodeTape. cbn - [Nat.eqb].
+                    destruct (Nat.eqb_spec 0 (sizeOfTape t1));
+                      destruct (eqb_spec 0 (maxSize)). all:try nia.
+         }
+         edestruct Terminates__mono as (?&?).
+         2:{ eexists. rewrite H. easy. }
+         cbn. set (tin:=midtape _ _ _).
+         eexists (select (putFirstAtEnd n) (t1:::v)), _.
+         assert (Ht1v:contains_tapes tin (select (putFirstAtEnd n) (t1 ::: v))). 
+         { hnf. subst tin. f_equal. unfold encode_tapes.
+           rewrite encode_list_concat.
+           autorewrite with list. cbn.  rewrite !concat_map,!map_map.
+           rewrite vector_to_list_correct,putFirstAtEnd_to_list.
+           autorewrite with list. cbn. repeat setoid_rewrite map_map.
+           rewrite concat_app;cbn. autorewrite with list. easy.
+         } split. easy.
+         split. 2:easy. hnf.
+         (do 2 eexists). split.
+         +intros ? ?. cbn in H. replace v0 with ((select (putFirstAtEnd n) (t1 ::: v))) in * by now eapply contains_tapes_inj. clear v0 H.
+          split. 1: {hnf. rewrite putEnd_invL. eauto. }
+          assert (H':=proj2_sig M2MBounds.Loop_steps_nice). hnf in H'.
+          unfold PrettyBounds.dominatedWith in H'.
+          rewrite H'. cbn in *. rewrite vector_to_list_correct, putFirstAtEnd_to_list.
+          rewrite BaseCode.encodeList_size_app,size_list, to_list_length.
+          unfold size. cbn - [mult plus].
+          autorewrite with list. cbn [length]. rewrite sizeOfTape_encodeTape_le.
+          erewrite sumn_map_le_pointwise with (f2:=fun x => _).
+          2:{ intros. rewrite sizeOfTape_encodeTape_le. rewrite sizeOfmTapes_upperBound. 2:now eapply tolist_In. reflexivity. }
+          rewrite !sumn_map_c,to_list_length.
+          reflexivity.
+         +cbn - [mult plus]. autorewrite with list;cbn - [plus mult].
+          rewrite length_concat,map_map;cbn - [plus mult];setoid_rewrite map_length.
+          rewrite sizeOfTape_encodeTape_le,Ht1.
+          rewrite sumn_le_bound.
+          2:{ intros ? (?&<-&?)%in_map_iff.
+              rewrite sizeOfTape_encodeTape_le, sizeOfmTapes_upperBound. 2:now apply tolist_In. reflexivity. }
+          rewrite map_length. rewrite to_list_length. [f__steps]:intros ? ? ?.
+          set (sizeOfmTapes _). unfold f__steps. reflexivity.
+        -intros (c__hs&t1&Hhd&Hsize&f&Hf). cbn - [mult plus] in *. inv Hhd. 
+         apply Realises__mono in Hf as (v0&v1&Hv0&Hv1&H__mono). cbn in Hv0.
+         hnf in H__mono;cbn in H__mono. unfold LiftTapes in H__mono;cbn in H__mono.
+         destruct H__mono as (outc&k&Hout&<-&_).
+         hnf in Hv0. revert Hv0. intros [= Htl].
+         unfold encode_tapes in Htl;rewrite encode_list_concat in Htl.
+         rewrite map_app,concat_map,map_map,vector_to_list_correct in Htl. cbn in Htl. 
+         setoid_rewrite map_map in Htl. rewrite <- !app_assoc in Htl. cbn in Htl.
+         assert (H':=Htl). eapply concat_eq_inv_borderL with (isBorder := fun c => c = inr sigList_cons) in H'. rewrite map_length,to_list_length in H'.
+         5:easy. 4:now cbn;intuition subst.
+         2,3:intros _ (x&<-&Hinx)%in_map_iff. 2,3:eexists _,_;split;[reflexivity | ].
+         2,3:now split;[easy | intros ? (y&<-&Hiny)%in_map_iff;easy].
+         destruct H' as [Hinit Hlast]. rewrite <- utils.map_skipn in Hlast.
+         destruct (split_vector v0 n) as (v'&vlst) eqn:Hsplit.
+         unshelve eassert (H':=split_vector_correct _ _). 6:rewrite Hsplit in H'. abstract nia.
+         cbn [fst snd] in H'.  apply (f_equal (@vector_to_list _ _ )) in H'. rewrite vector_to_list_cast in H'. clear Hsplit.
+         rewrite vector_app_to_list in H'.  
+         revert v' vlst H'. replace (Init.Nat.min n (S n)) with n by nia. replace (S n - n) with 1 by nia.
+         intros v' vlst eq. destruct (StepTM.destruct_vector1 vlst) as (ts&->). cbn in eq.
+         rewrite !vector_to_list_correct in eq.
+         rewrite <- eq in Hlast,Hinit.
+         replace v' with v in *.
+         2:{ eapply VectorSpec.eq_nth_iff. intros i ? <-.
+             unshelve eassert (Htmp:=Hinit (proj1_sig (Fin.to_nat i)) _). now destruct Fin.to_nat.
+             destruct (Fin.to_nat i) eqn:Hi.
+             rewrite <- !vector_to_list_correct,map_app,!vector_to_list_map,!vector_to_list_correct in Htmp. 
+             rewrite nth_error_app1 in Htmp. 2:now rewrite to_list_length.
+             cbn in Htmp. rewrite !vector_nth_error in Htmp.
+             destruct lt_dec. 2:easy. 
+             rewrite !nth_map' in Htmp. revert Htmp. intros [= Htmp].
+             apply map_injective in Htmp. 2:congruence. apply DecodeTape.tape_encode_injective in Htmp.
+             rewrite <- (Fin.of_nat_to_nat_inv i).  rewrite Hi;cbn.
+             erewrite Fin.of_nat_ext. apply Htmp.
+         }
+         clear Hinit v'.
+         rewrite skipn_app in Hlast. 2:now rewrite to_list_length. cbn in Hlast.
+         autorewrite with list in Hlast. cbn in Hlast. revert Hlast. intros [= ->].
+         exists ts. assert (Hts__size : sizeOfTape ts <= maxSize).
+         1:{ autorewrite with list in Hsize.  rewrite sizeOfTape_encodeTape in Hsize.
+             destruct (eqb_spec 0 maxSize);destruct sizeOfTape. all:cbn in Hsize;try nia. }
+         clear Hsize. split. easy. unfold initc in *. cbn in Hout.
+         unshelve eassert (Htmp := LiftTapes_lift _ _). 11:{ now rewrite Hout. } now apply putEndAtFirst_dupfree.
+         cbn in Htmp. unfold selectConf in Htmp. cbn in Htmp.
 
-Abort.
+         erewrite putEndAtFirst_to_list in Htmp. 2:exact eq.
+         eexists. setoid_rewrite loop_monotone. 2:eassumption. reflexivity. 
+         eapply H_HaltOrDiv. all:eassumption.
+    }
+    evar (time : nat -> nat). [time]:intros n0.
+    eexists.
+    { unfold f__steps, t__start. 
+      From Undecidability Require Import L.TM.TMflatComp.
+      Fail Intern.extractAs t. 
+      admit.
+
+    }
+
+  Admitted.
+
+End LMGenNP_to_TMGenNP_mTM.
